coqimp/framework/soundness/lemmas.v
@@ -21,6 +21,7 @@ Require Import Coq.Logic.FunctionalExtensionality.
 
 Open Scope nat.
 Open Scope code_scope.
+Open Scope mem_scope.
 
 (*+ Auxiliary Definition +*)
 Fixpoint indoms {tp : Type} (ls : list tp) M :=
@@ -192,6 +193,136 @@ Proof.
     }
 Qed.
 
+Lemma sep_reg_dec :
+  forall (s s' : SpReg),
+    {s = s'} + {s <> s'}.
+Proof.
+  intros.
+  destruct s; destruct s'; eauto;
+    try solve [right; intro; tryfalse].
+  destruct a; destruct a0; eauto;
+    try solve [right; intro; tryfalse].
+Qed.
+
+Lemma indom_nor_not :
+  forall (tp : Type) (l : tp) m,
+    {indom l m} + {~ indom l m}.
+Proof.
+  intros.
+  unfold indom.
+  destruct (m l); eauto.
+  right.
+  intro.
+  simpljoin1.
+  tryfalse.
+Qed.
+
+(*+ Lemmas for Integers +*)
+Lemma z_eq_to_int_eq :
+  forall z1 z2,
+    z1 = z2 -> $ z1 = $ z2.
+Proof.
+  intros.
+  subst; eauto.
+Qed.
+
+(*+ Lemmas for Memory +*)
+Lemma indom_merge_still :
+  forall (tp : Type) (l : tp) M m,
+    indom l M ->
+    indom l (merge M m).
+Proof.
+  intros.
+  unfold indom in *.
+  simpljoin1.
+  unfold merge in *.
+  destruct (M l) eqn:Heqe; eauto.
+  tryfalse.
+Qed.
+
+Lemma indom_merge_still2 :
+  forall (tp : Type) (l : tp) M m,
+    indom l m ->
+    indom l (merge M m).
+Proof.
+  intros.
+  unfold indom in *.
+  simpljoin1.
+  unfold merge in *.
+  destruct (M l) eqn:Heqe; eauto.
+Qed.
+
+Lemma indom_m2_disj_notin_m1 :
+  forall (tp : Type) (l : tp) m1 m2,
+    indom l m2 -> disjoint m1 m2 ->
+    ~ indom l m1.
+Proof.
+  intros.
+  intro.
+  unfold disjoint in *.
+  specialize (H0 l).
+  unfold indom in *.
+  simpljoin1.
+  rewrite H1 in H0.
+  rewrite H in H0; eauto.
+Qed.
+  
+Lemma indom_m1_disj_notin_m2 :
+  forall (tp : Type) (l : tp) m1 m2,
+    indom l m1 -> disjoint m1 m2 ->
+    ~ indom l m2.
+Proof.
+  intros.
+  intro.
+  unfold disjoint in *.
+  specialize (H0 l).
+  unfold indom in *.
+  simpljoin1.
+  rewrite H in H0.
+  rewrite H1 in H0; tryfalse.
+Qed.
+
+Lemma disj_merge_reverse_eq :
+  forall (tp : Type) (m1 m2 : tp -> option Word),
+    disjoint m1 m2 ->
+    merge m1 m2 = merge m2 m1.
+Proof.
+  intros.
+  eapply functional_extensionality.
+  intros.
+  unfold merge in *.
+  destruct (m1 x) eqn:Heqe1;
+    destruct (m2 x) eqn:Heqe2; simpl; eauto; tryfalse.
+  unfold disjoint in *.
+  specialize (H x).
+  rewrite Heqe1 in H;
+    rewrite Heqe2 in H; tryfalse.
+Qed.
+
+Lemma disj_sym :
+  forall (tp : Type) (m1 m2 : tp -> option Word),
+    disjoint m1 m2 -> disjoint m2 m1.
+Proof.
+  intros.
+  unfold disjoint in *.
+  intros.
+  specialize (H x).
+  destruct (m1 x) eqn:Heqe1;
+    destruct (m2 x) eqn:Heqe2; tryfalse; eauto.
+Qed.
+
+Lemma indom_isindom :
+  forall (tp : Type) (l : tp) m,
+    indom l m -> is_indom l m = true.
+Proof.
+  intros.
+  unfolds.
+  unfold indom in H.
+  simpljoin1.
+  rewrite H.
+  eauto.
+Qed.
+
 (*+ Lemmas about register state +*)
 Definition dom_eq {tp : Type} (M m : tp -> option Word) :=
   (forall l, indom l M -> indom l m) /\ (forall l, indom l m -> indom l M).
@@ -209,6 +340,1783 @@ Proof.
 
   unfolds RegMap.set.
   destruct_rneq.
+Qed.
+
+Lemma indom_setR_eq_RegMap_set :
+  forall (s : RegName) R w,
+    indom s R ->
+    set_R R s w = RegMap.set s (Some w) R.
+Proof.
+  intros.
+  unfold set_R.
+  unfold is_indom.
+  destruct (R s) eqn:Heqe; eauto.
+  unfold indom in H.
+  simpljoin1.
+  rewrite H in Heqe.
+  tryfalse.
+Qed.
+
+Lemma regset_l_l_indom :
+  forall rn v m,
+    indom rn (RegMap.set rn (Some v) m).
+Proof.
+  intros.
+  unfold indom.
+  exists v.
+  unfolds RegMap.set.
+  destruct_rneq.
+Qed.
+
+Lemma regset_twice :
+  forall (A : Type) l (v v1 : A) m,
+    RegMap.set l (Some v) (RegMap.set l (Some v1) m) =
+    RegMap.set l (Some v) m.
+Proof.
+  intros.
+  eapply functional_extensionality.
+  intro.
+  unfolds RegMap.set.
+  destruct_rneq.
+Qed.
+
+Lemma not_indom_set_R_stable :
+  forall s R w,
+    ~ indom s R ->
+    set_R R s w = R.
+Proof.
+  intros.
+  unfolds set_R.
+  unfold is_indom.
+  destruct (R s) eqn:Heqe; eauto.
+  false.
+  eapply H; eauto.
+  unfold indom.
+  eauto.
+Qed.
+
+Lemma indom_setR_merge_eq :
+  forall M m l v,
+    indom l M ->
+    RegMap.set l (Some v) (merge M m) = merge (RegMap.set l (Some v) M) m.
+Proof.
+  intros.
+  unfold RegMap.set, merge in *.
+  eapply functional_extensionality.
+  intro.
+  unfold indom in *.
+  simpljoin1. 
+  destruct_rneq.
+Qed.
+
+Lemma indom_setR_merge_eq1 :
+  forall (R : RegFile) M (rn : RegName) m v,
+    indom rn M ->
+    set_R (merge M m) rn v = merge (set_R M rn v) m.
+Proof.
+  intros.
+  unfolds set_R.
+  unfold is_indom.
+  destruct ((M ⊎ m) rn) eqn:Heqe.
+  {
+    destruct (M rn) eqn:Heqe1; eauto.
+    unfold RegMap.set.
+    eapply functional_extensionality; eauto.
+    intro.
+    destruct_rneq.
+    unfold merge.
+    subst. 
+    destruct_rneq.
+    unfold merge.
+    destruct (M x) eqn:Heqe2; eauto.
+    destruct_rneq.
+    destruct_rneq.
+    false.
+    unfold indom in *.
+    simpljoin1.
+    rewrite H in Heqe1.
+    tryfalse.
+  }
+  {
+    false.
+    unfold indom in *.
+    simpljoin1.
+    unfold merge in *.
+    rewrite H in Heqe.
+    tryfalse.
+  }
+Qed.
+  
+Lemma indom_setR_merge_eq2 :
+  forall (R : RegFile) M (rn : RegName) m v,
+    ~ indom rn M -> disjoint M m ->
+    set_R (merge M m) rn v = merge M (set_R m rn v).
+Proof. 
+  intros.
+  unfolds set_R.
+  unfold is_indom.
+  destruct ((M ⊎ m) rn) eqn:Heqe.
+  {
+    destruct (m rn) eqn:Heqe1.
+    unfold RegMap.set.
+    eapply functional_extensionality.
+    intros.
+    destruct_rneq.
+    subst.
+    unfold merge.
+    destruct (M rn) eqn:Heqe2; eauto.
+    false.
+    eapply H.
+    unfold indom; eauto.
+    destruct_rneq.
+    unfold merge.
+    destruct (M x) eqn:Heqe2; eauto.
+    destruct_rneq.
+    false.
+    unfold merge in Heqe.
+    destruct (M rn) eqn:Heqe2; tryfalse.
+    eapply H.
+    unfold indom; eauto.
+  }
+  {
+    destruct (m rn) eqn:Heqe1.
+    {
+      unfold merge in *.
+      destruct (M rn) eqn:Heqe2; tryfalse.
+    }
+    {
+      eauto.
+    }
+  }
+Qed.
+
+Lemma disjoint_setR_still1:
+  forall (m1 m2 : RegFile) (rn : RegName) (v : Word),
+    disjoint m1 m2 ->
+    disjoint (set_R m1 rn v) m2.
+Proof.
+  intros.
+  unfold disjoint in *.
+  intro.
+  specialize (H x).
+  unfold set_R.
+  destruct (m1 x) eqn:Heqe1.
+  {
+    unfold is_indom.
+    destruct (m1 rn) eqn:Heqe2.
+    unfold RegMap.set.
+    destruct_rneq.
+    rewrite Heqe1.
+    destruct (m2 x) eqn:Heqe3.
+    tryfalse.
+    eauto.
+    rewrite Heqe1.
+    eauto.
+  }
+  {
+    unfold is_indom.
+    destruct (m1 rn) eqn:Heqe2.
+    unfold RegMap.set.
+    destruct_rneq.
+    rewrite Heqe1.
+    eauto.
+    rewrite Heqe1.
+    eauto.
+  }
+Qed.
+  
+Lemma disjoint_setR_still2:
+  forall (m1 m2 : RegFile) (rn : RegName) (v : Word),
+    disjoint m1 m2 ->
+    disjoint m1 (set_R m2 rn v).
+Proof.
+  intros.
+  unfold disjoint in *.
+  intros.
+  specialize (H x).
+  unfold set_R.
+  destruct (m1 x) eqn:Heqe1.
+  {
+    destruct (is_indom rn m2) eqn:Heqe2; tryfalse.
+    {
+      destruct (m2 x) eqn:Heqe3.
+      unfold RegMap.set.
+      destruct_rneq.
+      unfold RegMap.set.
+      destruct_rneq.
+      unfold is_indom in *.
+      subst.
+      rewrite Heqe3 in Heqe2; tryfalse.
+      rewrite Heqe3; eauto.
+    }
+    {
+      destruct (m2 x) eqn:Heqe3; tryfalse.
+      eauto.
+    }
+  }
+  {
+    destruct (is_indom rn m2) eqn:Heqe2; tryfalse.
+    {
+      unfold is_indom in *.
+      unfold RegMap.set in *.
+      destruct_rneq.
+    }
+    {
+      eauto.
+    }
+  }
+Qed.
+
+(*+ Lemmas about Sep Star +*)
+Lemma sep_star_split :
+  forall s p1 p2,
+    s |= p1 ** p2 ->
+    exists s1 s2, s1 |= p1 /\ s2 |= p2 /\ state_union s1 s2 s.
+Proof.
+  intros.
+  simpl in H.
+  simpljoin1; eauto.
+Qed.
+
+Ltac sep_star_split_tac :=
+  match goal with
+  | H : _ |= ?p1 ** ?p2 |- _ =>
+    let x := fresh in
+    let x1 := fresh in
+    eapply sep_star_split in H;
+    destruct H as [ x [x1 H] ]; simpljoin1;
+    destruct_state x; destruct_state x1;
+    sep_star_split_tac
+  | _ => idtac
+  end.
+
+(*+ Lemmas for delay list +*)
+Lemma not_in_exe_dly_stable :
+  forall D R R' D' s,
+    exe_delay R D = (R', D') ->
+    ~ In s (getRegs D) ->
+    ~ In s (getRegs D').
+Proof.
+  intro D.
+  induction D; intros.
+  -
+    simpl in H.
+    inversion H; subst.
+    intro.
+    simpls.
+    tryfalse.
+  -
+    destruct a, p.
+    simpl in H.
+    destruct d.
+    {
+      destruct (exe_delay R D) eqn:Heqe1; eauto.
+      inversion H; subst.
+      eapply IHD in Heqe1; eauto.
+      intro.
+      eapply H0.
+      simpl.
+      eauto.
+    }
+    {
+      destruct (exe_delay R D) eqn:Heqe1; eauto.
+      inversion H; subst.
+      eapply IHD with (s := s) in Heqe1; eauto.
+      intro.
+      simpl in H1.
+      destruct H1; subst.
+      eapply H0.
+      simpl; eauto.
+      eapply Heqe1; eauto.
+      intro.
+      eapply H0.
+      simpl; eauto.
+    }
+Qed.
+
+Lemma dlyitem_in_dlyls_reg_in :
+  forall D t s w,
+    In (t, s, w) D ->
+    In s (getRegs D).
+Proof.
+  intro D.
+  induction D; intros.
+  -
+    simpls; eauto.
+  -
+    destruct a, p.
+    simpl in H.
+    destruct H.
+    inversion H; subst.
+    simpl; eauto.
+    simpl.
+    right.
+    eauto.
+Qed.
+
+Lemma dlytime_gt_zero_exe_still :
+  forall D t s w D' R R',
+    In (S t, s, w) D -> (R', D') = exe_delay R D ->
+    In (t, s, w) D'.
+Proof.
+  intro D.
+  induction D; intros.
+  -
+    simpl in H0.
+    inversion H0; subst.
+    simpl in H.
+    tryfalse.
+  -
+    destruct a, p.
+    simpl in H.
+    destruct H.
+    {
+      inversion H; subst.
+      simpl in H0. 
+      destruct (exe_delay R D) eqn:Heqe; eauto.
+      inversion H0; subst.
+      simpl; eauto.
+    }
+    {
+      simpl in H0.
+      destruct n.
+      {
+        destruct (exe_delay R D) eqn:Heqe; eauto.
+        inversion H0; subst.
+        symmetry in Heqe.
+        eapply IHD in Heqe; eauto.
+      }
+      {
+        destruct (exe_delay R D) eqn:Heqe; eauto.
+        inversion H0; subst.
+        symmetry in Heqe.
+        eapply IHD in Heqe; eauto.
+        simpl; eauto.
+      }
+    }
+Qed.
+    
+Lemma noDup_exe_dly_stable :
+  forall D R R' D',
+    noDup (getRegs D) ->
+    exe_delay R D = (R', D') ->
+    noDup (getRegs D').
+Proof.
+  intro D.
+  induction D; intros.
+  -
+    simpl in H0.
+    inversion H0; subst.
+    econstructor; eauto.
+  -
+    destruct a, p.
+    simpl in H0.
+    destruct d.
+    {
+      destruct (exe_delay R D) eqn:Heqe.
+      inversion H0; subst.
+      simpl in H.
+      inversion H; subst.
+      eauto.
+    }
+    {
+      destruct (exe_delay R D) eqn:Heqe.
+      inversion H0; subst.
+      simpl in H.
+      inversion H; subst.
+      simpl.
+      econstructor; eauto.
+      eapply not_in_exe_dly_stable; eauto.
+    }
+Qed.
+
+Lemma regdlySt_dly_nil_false :
+  forall n s w M R F,
+    regdlySt n s w (M, (R, F), []) -> False.
+Proof.
+  intro n.
+  induction n; intros.
+  -
+    simpls.
+    unfolds inDlyBuff.
+    simpljoin1.
+    simpls; tryfalse.
+  -
+    simpl in H.
+    destruct H.
+    unfolds inDlyBuff.
+    simpljoin1.
+    simpls.
+    tryfalse.
+    eauto.
+Qed.
+
+Lemma regdlySt_dlyls_relevent :
+  forall t D s w M M' R R' F F',
+    regdlySt t s w (M, (R, F), D) ->
+    regdlySt t s w (M', (R', F'), D).
+Proof.
+  intro t.
+  induction t; intros.
+  -
+    unfolds regdlySt.
+    simpls.
+    eauto.
+  -
+    simpls.
+    destruct H; eauto.
+Qed.
+    
+Lemma dly_reduce_Aemp_stable :
+  forall D M R R' F D',
+    (M, (R, F), D) |= Aemp -> (R', D') = exe_delay R D ->
+    (M, (R', F), D') |= Aemp.
+Proof.
+  intros D.
+  induction D; intros.
+  -
+    simpls.
+    inversion H0; eauto.
+  -
+    destruct a, p.
+    assert ((M, (R, F), D) |= Aemp).
+    {
+      clear - H.
+      simpls; eauto.
+    }
+
+    simpl in H0.
+    destruct d.
+    {
+      destruct (exe_delay R D) eqn:Heqe; eauto.
+      inversion H0; subst.
+      eapply IHD with (R' := r) (D' := d) in H1; eauto.
+      simpl in H.
+      simpljoin1.
+      simpls.
+      simpljoin1.
+      split; eauto.
+    }
+    {
+      destruct (exe_delay R D) eqn:Heqe; eauto.
+      inversion H0; subst.
+      eapply IHD with (R' := r) (D' := d0) in H1; eauto.
+    }
+Qed.
+
+Lemma dly_reduce_Amapsto_stable :
+  forall D M R R' F D' a w,
+    (M, (R, F), D) |= a |-> w -> (R', D') = exe_delay R D ->
+    (M, (R', F), D') |= a |-> w.
+Proof.
+  intros D.
+  induction D; intros.
+  -
+    simpls.
+    inversion H0; eauto.
+  -
+    destruct a, p.
+    assert ((M, (R, F), D) |= a0 |-> w).
+    {
+      clear - H.
+      simpls.
+      eauto.
+    }
+
+    simpl in H0.
+    destruct d.
+    {
+      destruct (exe_delay R D) eqn:Heqe.
+      inversion H0; subst.
+      eapply IHD with (R' := r) (D' := d) in H1; eauto.
+      simpls.
+      simpljoin1; eauto.
+    }
+    {
+      destruct (exe_delay R D) eqn:Heqe.
+      inversion H0; subst.
+      eapply IHD with (R' := r) (D' := d0) in H1; eauto.
+    }
+Qed.
+
+Lemma dly_reduce_Aaexp_stable :
+  forall D M R R' F D' a a0,
+    (M, (R, F), D) |= a ==ₓ a0 -> (R', D') = exe_delay R D ->
+    (M, (R', F), D') |= a ==ₓ a0.
+Proof.
+  intros D.
+  induction D; intros.
+  -
+    simpls.
+    simpljoin1.
+    eauto.
+  -
+    destruct a, p.
+    assert ((M, (R, F), D) |= a0 ==ₓ a1).
+    {
+      clear - H.
+      simpls.
+      eauto.
+    }
+
+    simpl in H0.
+    destruct d.
+    {
+      destruct (exe_delay R D) eqn:Heqe.
+      inversion H0; subst.   
+      eapply IHD with (R' := r) (D' := d) in H1; eauto.
+      clear - H1.
+      simpls.
+      simpljoin1.
+      unfolds eval_addrexp.
+      destruct a0; eauto.
+      split; eauto.
+
+      unfolds eval_opexp.
+      destruct o; eauto.
+      unfold set_R.
+      unfold is_indom.
+      destruct (r s) eqn :Heqe; eauto.
+      unfolds RegMap.set.
+      destruct_rneq; eauto.
+      unfold set_R.
+      unfold is_indom.
+      destruct (r s) eqn:Heqe; eauto.
+      unfold RegMap.set.
+      destruct_rneq; eauto.
+      destruct (r g) eqn:Heqe2; eauto.
+      unfolds eval_opexp.
+      destruct o; eauto.
+      destruct_rneq; eauto.
+    }
+    {
+      destruct (exe_delay R D) eqn:Heqe; subst.
+      inversion H0; subst.
+      eapply IHD with (R' := r) (D' := d0) in H1; eauto.
+    }
+Qed.
+
+Lemma dly_reduce_Aoexp_stable :
+  forall D M R R' F D' o w,
+    (M, (R, F), D) |= o ==ₑ w -> (R', D') = exe_delay R D ->
+    (M, (R', F), D') |= o ==ₑ w.
+Proof.
+  intros D.
+  induction D; intros.
+  -
+    simpl in H0.
+    inversion H0; eauto.
+  -
+    destruct a, p.
+    assert ((M, (R, F), D) |= o ==ₑ w).
+    {
+      clear - H.
+      simpls.
+      eauto.
+    }
+
+    simpl in H0.
+    destruct d.
+    {
+      destruct (exe_delay R D) eqn:Heqe; eauto.
+      inversion H0; subst.
+      eapply IHD with (R' := r) (D' := d) in H1; eauto.
+      clear - H1.
+      simpls.
+      unfolds eval_opexp.
+      destruct o; eauto.
+      unfolds set_R.
+      unfold is_indom.
+      destruct (r s); eauto.
+      unfolds RegMap.set.
+      destruct_rneq; eauto.
+    }
+    {
+      destruct (exe_delay R D) eqn:Heqe; eauto.
+      inversion H0; subst.
+      eapply IHD with (R' := r) (D' := d0) in H1; eauto.
+    }
+Qed.
+
+Lemma dly_reduce_reg_stable :
+  forall D M R R' F D' r w,
+    (M, (R, F), D) |= r |=> w -> (R', D') = exe_delay R D ->
+    (M, (R', F), D') |= r |=> w.
+Proof.
+  intro D.
+  induction D; intros.
+  -
+    simpls.
+    inversion H0; eauto.
+  -
+    destruct a, p.
+    assert ((M, (R, F), D) |= r |=> w).
+    {
+      clear - H.
+      simpls.
+      unfolds regSt.
+      simpljoin1; eauto.
+      simpls.
+      repeat (split; eauto).
+      intro.
+      eapply H1.
+      clear - H2.
+      unfolds regInDlyBuff.
+      destruct r; eauto; tryfalse.
+      simpls.
+      eauto.
+    }
+
+    simpl in H0.
+    destruct d.
+    {
+      destruct (exe_delay R D) eqn:Heqe.
+      inversion H0; subst. 
+      eapply IHD with (R' := r0) (D' := d) in H1; eauto.
+      clear - H1 H.
+      simpls.
+      unfolds regSt.
+      simpls.
+      simpljoin1.
+      repeat (split; eauto).
+      unfold set_R.
+      unfold is_indom.
+      unfold RegMap.set.
+      destruct_rneq.
+      subst.
+      false.
+      eapply H4.
+      unfold regInDlyBuff.
+      simpl; eauto.
+    }
+    {
+      destruct (exe_delay R D) eqn:Heqe.
+      inversion H0; subst.
+      eapply IHD with (R' := r0) (D' := d0) in H1; eauto.
+      clear - H H1.
+      simpls.
+      unfolds regSt.
+      simpls.
+      simpljoin1; eauto.
+      repeat (split; eauto).
+      intro. 
+      eapply H2.
+      clear - H H4.
+      unfolds regInDlyBuff.
+      destruct r; eauto; tryfalse.
+      simpls; eauto.
+      destruct H; eauto.
+      subst.
+      false.
+      eapply H4; eauto.
+    }
+Qed.
+
+Lemma reg_not_in_dlybuff_exe_dly_stable :
+  forall D D' R' (s : SpReg) v,
+    exe_delay (RegMap.set s (Some v) empR) D = (R', D') ->
+    ~ In s (getRegs D) ->
+    R' = RegMap.set s (Some v) empR.
+Proof.
+  intro D.
+  induction D; intros.
+  -
+    simpl in H.
+    inversion H; eauto.
+  -
+    destruct a, p.
+    simpl in H0.
+    simpl in H.
+    destruct d.
+    {
+      destruct (exe_delay (RegMap.set s (Some v) empR) D) eqn:Heqe.
+      inversion H; subst.
+      eapply IHD in Heqe; eauto.
+      subst.
+ 
+      unfold set_R.
+      unfold is_indom.
+      unfold RegMap.set.
+      destruct (sep_reg_dec s0 s); tryfalse.
+      {
+        false.
+        eapply H0; eauto.
+      }
+      {
+        destruct_rneq.
+      }
+    }
+    {
+      destruct (exe_delay (RegMap.set s (Some v) empR) D) eqn:Heqe; eauto.
+      inversion H; subst.
+      eapply IHD in Heqe; eauto.
+    }
+Qed.
+    
+Lemma dlytime_zero_exe_dly :
+  forall D M R R' F D' s w,
+    (M, (R, F), D) |= 0 @ s |==> w ->
+    (R', D') = exe_delay R D ->
+    (M, (R', F), D') |= s |=> w.
+Proof.
+  intro D.
+  induction D; intros.
+  -
+    simpl in H.
+    simpljoin1.
+    destruct H2.
+    {
+      unfolds inDlyBuff.
+      simpljoin1.
+      simpl in H.
+      tryfalse.
+    }
+    {
+      simpl in H0.
+      inversion H0; subst.
+      unfolds regSt.
+      simpls.
+      simpljoin1.
+      eapply equal_f in H.
+      assert (RegMap.set s (Some x) empR s = RegMap.set s (Some w) empR s); eauto.
+      clear - H.
+      unfold RegMap.set in H.
+      destruct_rneq_H.
+      inversion H; subst.
+      unfold regSt.
+      simpl; eauto.
+    }
+  - 
+    destruct a, p.
+    simpl in H0. 
+    destruct d.
+    {
+      destruct (exe_delay R D) eqn:Heqe.
+      inversion H0; subst.
+
+      lets Ht : H.
+      simpl in Ht.
+      simpljoin1.
+      destruct H3.
+      {
+        unfolds inDlyBuff.
+        simpljoin1.
+        simpl in H0.
+        destruct H0.
+        { 
+          inversion H0; subst.
+          simpl in H1.
+          inversion H1; subst.
+          lets Hexe_dly : Heqe.
+          eapply reg_not_in_dlybuff_exe_dly_stable in Heqe; eauto.
+          subst.
+          simpl.
+          unfold regSt.
+          simpl.
+          repeat (split; eauto).
+          rewrite indom_setR_eq_RegMap_set; eauto.
+          rewrite regset_twice; eauto.
+          eapply regset_l_l_indom; eauto.
+          eapply not_in_exe_dly_stable; eauto.
+        }
+        {
+          inversion H1; subst.
+          assert (s <> s0).
+          {
+            intro.
+            subst.
+            eapply dlyitem_in_dlyls_reg_in in H0; eauto.
+          }
+
+          assert ((empM, (RegMap.set s (Some x) empR, F), D) |= 0 @ s |==> w).
+          {
+            clear - H H2.
+            simpls.
+            simpljoin1.
+            destruct H1.
+            unfold inDlyBuff in H0.
+            simpljoin1.
+            simpl in H0.
+            destruct H0.
+            inversion H0; subst; tryfalse.
+            exists x.
+            repeat (split; eauto).
+            left.
+            unfold inDlyBuff.
+            simpl in H1.
+            inversion H1; eauto.
+            exists x.
+            repeat (split; eauto).
+            right.
+            unfolds regSt.
+            simpls.
+            simpljoin1; eauto.
+            repeat (split; eauto).
+          }
+
+          eapply IHD with (R' := r) (D' := d) in H3; eauto.
+          clear - H2 H3.
+          simpls.
+          unfolds regSt.
+          simpls.
+          simpljoin1.
+          repeat (split; eauto).
+          unfold set_R.
+          unfold is_indom.
+          unfold RegMap.set at 1.
+          destruct_rneq.
+        }
+      }
+      {
+        assert ((empM, (RegMap.set s (Some x) empR, F), D) |= 0 @ s |==> w).
+        { 
+          clear - H0.
+          simpl.
+          exists x.
+          repeat (split; eauto).
+          right.
+          unfolds regSt.
+          simpls.
+          simpljoin1.
+          repeat (split; eauto).
+        }
+
+        eapply IHD with (R' := r) (D' := d) in H1; eauto.
+
+        assert (s <> s0).
+        {
+          clear - H0.
+          unfolds regSt.
+          simpls.
+          simpljoin1.
+          intro.
+          eapply H1; eauto.
+        }
+
+        clear - H1 H2.
+        simpls.
+        unfolds regSt.
+        simpls.
+        simpljoin1.
+        repeat (split; eauto).
+        unfold set_R.
+        unfold is_indom.
+        unfold RegMap.set.
+        destruct_rneq.
+      }
+    }
+    {
+      destruct (exe_delay R D) eqn:Heqe.
+      inversion H0; subst.
+
+      assert ((M, (R, F), D) |= 0 @ s |==> w).
+      {
+        clear - H.
+        simpls.
+        simpljoin1.
+        exists x.
+        repeat (split; eauto).
+        destruct H1.
+        {
+          unfolds inDlyBuff.
+          simpljoin1.
+          simpl in H.
+          destruct H.
+          inversion H.
+          inversion H0; subst; eauto.
+        }
+        {
+          right.
+          unfolds regSt.
+          simpls.
+          simpljoin1.
+          repeat (split; eauto).
+        }
+      }
+
+      eapply IHD with (R' := r) (D' := d0) in H1; eauto.
+
+      assert (s <> s0).
+      { 
+        clear - H.
+        intro.
+        subst.
+        simpls.
+        simpljoin1.
+        destruct H1.
+        unfolds inDlyBuff.
+        simpls; simpljoin1.
+        destruct H.
+        inversion H; tryfalse.
+        inversion H0; subst.
+        eapply dlyitem_in_dlyls_reg_in in H; eauto.
+        unfolds regSt.
+        simpls.
+        simpljoin1.
+        eauto.
+      }
+
+      clear - H1 H2.
+      simpls.
+      unfolds regSt.
+      simpls.
+      simpljoin1.
+      repeat (split; eauto).
+      intro.
+      destruct H; tryfalse.
+    }
+Qed.
+
+Lemma regst_conseq_regdly :
+  forall M R F D t (s : SpReg) w,
+    (M, (R, F), D) |= s |=> w ->
+    (M, (R, F), D) |= t @ s |==> w.
+Proof.
+  intros.
+  simpls.
+  unfolds regSt.
+  simpls.
+  simpljoin1.
+  exists w.
+  repeat (split; eauto).
+Qed.
+
+Lemma regdlySt_dlycons_stable :
+  forall t t0 s s0 w w0 M R F D,
+    regdlySt t s w (M, (R, F), D) -> ~ In s0 (getRegs D) ->
+    regdlySt t s w (M, (R, F), (t0, s0, w0) :: D).
+Proof.
+  intro t.
+  induction t; intros.
+  -
+    simpls.
+    unfolds inDlyBuff.
+    simpls.
+    simpljoin1.
+    split; eauto.
+    econstructor; eauto.
+  -
+    simpls.
+    destruct H.
+    {
+      left.
+      unfolds inDlyBuff.
+      simpljoin1.
+      simpl; eauto.
+      split; eauto.
+      econstructor; eauto.
+    }
+    {
+      right.
+      eauto.
+    }
+Qed.
+
+Lemma dlytm_gt_zero_exe_dly :
+  forall D R' D' F x t (s : SpReg) w,
+    (R', D') = exe_delay (RegMap.set s (Some x) empR) D ->
+    inDlyBuff (S t, s, w) D ->
+    (empM, (R', F), D') |= t @ s |==> w.
+Proof.
+  intro D.
+  induction D; intros.
+  -
+    unfolds inDlyBuff.
+    simpls.
+    simpljoin1; tryfalse.
+  -
+    destruct a, p.
+    unfold inDlyBuff in H0.
+    simpljoin1.
+    simpl in H0. 
+    destruct H0.
+    {
+      inversion H0; subst.
+      simpl in H1.
+      simpl in H.
+      destruct (exe_delay (RegMap.set s (Some x) empR) D) eqn:Heqe.
+      inversion H; subst.
+      inversion H1; subst.
+      lets Ht : Heqe.
+      eapply reg_not_in_dlybuff_exe_dly_stable in Heqe; eauto.
+      subst.
+      simpl.
+      exists x.
+      repeat (split; eauto).
+      left.
+      destruct t; simpl; eauto.
+      unfold inDlyBuff.
+      simpl; eauto.
+      split; eauto.
+      econstructor; eauto.
+      eapply not_in_exe_dly_stable; eauto.
+      eapply noDup_exe_dly_stable; eauto.
+
+      left.
+      unfold inDlyBuff.
+      split; simpl; eauto.
+      econstructor; eauto.
+      eapply not_in_exe_dly_stable; eauto.
+      eapply noDup_exe_dly_stable; eauto.
+    }
+    {
+      simpl in H.
+      destruct d.
+      {  
+        destruct (exe_delay (RegMap.set s (Some x) empR) D) eqn:Heqe.
+        inversion H; subst.
+        symmetry in Heqe.
+        lets Ht : Heqe.
+        eapply IHD with (t := t) (w := w) (F := F) in Heqe; eauto.
+        Focus 2.
+        unfold inDlyBuff.
+        simpl in H1.
+        inversion H1; subst; eauto.
+        eapply dlytime_gt_zero_exe_still in Ht; eauto.
+        clear - Heqe Ht.
+        simpl in Heqe.
+        simpljoin1.
+        destruct H1.
+        {
+          simpl.
+          destruct (sep_reg_dec s s0).
+          {
+            subst.
+            exists w0.
+            repeat (split; eauto).
+            unfold set_R.
+            unfold is_indom.
+            unfolds RegMap.set.
+            destruct_rneq.
+            eapply functional_extensionality; eauto.
+            intros.
+            destruct_rneq.
+            left.
+            eapply regdlySt_dlyls_relevent; eauto.
+          }
+          {
+            exists x.
+            repeat (split; eauto).
+            unfold set_R.
+            unfold is_indom.
+            unfold RegMap.set.
+            destruct_rneq.
+            left.
+            eapply regdlySt_dlyls_relevent; eauto.
+          }
+        }
+        
+        unfolds regSt.
+        simpls.
+        simpljoin1.
+        eapply dlyitem_in_dlyls_reg_in in Ht; eauto.
+        tryfalse.
+      }
+      {
+        destruct (exe_delay (RegMap.set s (Some x) empR) D) eqn:Heqe.
+        inversion H; subst.
+        symmetry in Heqe.
+
+        assert (s <> s0).
+        {
+          clear - H0 H1.
+          intro.
+          subst.
+          simpl in H1.
+          inversion H1; subst.
+          eapply dlyitem_in_dlyls_reg_in in H0; eauto.
+        }
+
+        lets Ht : Heqe. 
+        eapply IHD with (t := t) (w := w) (F := F) in Heqe; eauto.
+        Focus 2. 
+        clear - H0 H1.
+        unfold inDlyBuff.
+        simpl in H1.
+        inversion H1; eauto.
+
+        simpl in H1. 
+        inversion H1; subst. 
+        clear - Heqe H2 H5 Ht.
+        simpls.
+        simpljoin1.
+        exists x0.
+        repeat (split; eauto).
+        destruct H1.
+        left.
+        eapply regdlySt_dlycons_stable; eauto.
+        eapply not_in_exe_dly_stable; eauto.
+        right.
+        clear - H H2.
+        unfolds regSt.
+        simpls.
+        simpljoin1.
+        repeat (split; eauto).
+        intro.
+        destruct H0; subst; tryfalse.
+      }
+    }
+Qed.
+
+Lemma regdlySt_in_vl_eq :
+  forall t s0 w w0 M R F D,
+    regdlySt t s0 w (M, (R, F), (0, s0, w0) :: D) ->
+    w = w0.
+Proof.
+  intro t.
+  induction t; intros.
+  -
+    simpl in H.
+    unfolds inDlyBuff.
+    simpljoin1.
+    simpl in H.
+    destruct H.
+    inversion H; eauto.
+    simpl in H0.
+    inversion H0; subst.
+    eapply dlyitem_in_dlyls_reg_in in H; eauto.
+    tryfalse.
+  - 
+    simpl in H.
+    destruct H.
+    {
+      unfolds inDlyBuff.
+      simpljoin1.
+      simpl in H.
+      destruct H.
+      inversion H; tryfalse.
+      simpl in H0.
+      inversion H0; subst.
+      eapply dlyitem_in_dlyls_reg_in in H; eauto.
+      tryfalse.
+    }
+    {
+      eauto.
+    }
+Qed.
+
+Lemma regdlySt_noDup :
+  forall t s w M R F D,
+    regdlySt t s w (M, (R, F), D) ->
+    noDup (getRegs D).
+Proof.
+  intro t.
+  induction t; intros.
+  -
+    simpls.
+    unfolds inDlyBuff.
+    simpljoin1.
+    eauto.
+  -
+    simpl in H.
+    destruct H.
+    unfolds inDlyBuff.
+    simpljoin1.
+    eauto.
+    eauto.
+Qed.
+
+Lemma regdlySt_cons_notin :
+  forall t t' s w M R F D w0,
+    regdlySt t s w (M, (R, F), (t', s, w0) :: D) ->
+    ~ In s (getRegs D).
+Proof.
+  intro t.
+  induction t; intros.
+  -
+    simpl in H.
+    unfolds inDlyBuff.
+    simpls.
+    simpljoin1.
+    inversion H0; subst.
+    eauto.
+  -
+    simpls.
+    destruct H.
+    {
+      unfolds inDlyBuff.
+      simpls.
+      simpljoin1.
+      inversion H0; subst.
+      eauto.
+    }
+    {
+      eapply regdlySt_noDup in H; eauto.
+      simpl in H.
+      inversion H; eauto.
+    }
+Qed.
+
+
+Lemma regdlySt_noteq_cons_remove :
+  forall t t' s s' w w' M R F D,
+    regdlySt t s w (M, (R, F), (t', s', w') :: D) ->
+    s <> s' ->
+    regdlySt t s w (M, (R, F), D).
+Proof.
+  intro t.
+  induction t; intros.
+  -
+    simpls.
+    unfolds inDlyBuff.
+    simpljoin1.
+    simpl in H.
+    destruct H.
+    inversion H; subst.
+    tryfalse.
+    simpl in H1.
+    inversion H1; eauto.
+  -
+    simpls.
+    destruct H.
+    {
+      unfolds inDlyBuff.
+      simpls.
+      simpljoin1.
+      destruct H.
+      inversion H; subst.
+      tryfalse.
+      left.
+      inversion H1; subst; eauto.
+    }
+    {
+      eauto.
+    }
+Qed.
+
+Lemma regdlySt_cons_noteq_stable :
+  forall t s w s0 d w0 M R F D,
+    regdlySt t s w (M, (R, F), D) -> s <> s0 -> ~ In s0 (getRegs D) ->
+    regdlySt t s w (M, (R, F), (d, s0, w0) :: D).
+Proof.
+  intro t.
+  induction t; intros.
+  -
+    simpls.
+    unfolds inDlyBuff.
+    simpljoin1.
+    simpl.
+    split; eauto.
+    econstructor; eauto.
+  -
+    simpls.
+    destruct H.
+    {
+      left.
+      unfolds inDlyBuff.
+      simpls.
+      split; eauto.
+      simpljoin1; eauto.
+      econstructor; eauto.
+      simpljoin1; eauto.
+    }
+    {
+      right.
+      eauto.
+    }
+Qed.
+
+Lemma regdlySt_cons_same :
+  forall t s w M R F D,
+    noDup (s :: getRegs D) ->
+    regdlySt t s w (M, (R, F), (t, s, w) :: D).
+Proof.
+  intros.
+  destruct t.
+  {
+    simpls.
+    unfold inDlyBuff.
+    simpl; eauto.
+  }
+  {
+    simpl.
+    left.
+    unfold inDlyBuff.
+    simpl; eauto.
+  }
+Qed.
+  
+Lemma regdlySt_dlytim_reduce_stable :
+  forall t s w M R F D d w0,
+    regdlySt t s w (M, (R, F), (S d, s, w0) :: D) ->
+    regdlySt t s w (M, (R, F), (d, s, w0) :: D).
+Proof.
+  intro t.
+  induction t; intros.
+  -
+    simpls.
+    unfolds inDlyBuff.
+    simpljoin1.
+    simpl in H.
+    destruct H.
+    inversion H; subst.
+    simpl in H0.
+    inversion H0; subst; eauto.
+    simpl.
+    repeat (split; eauto).
+  -
+    simpls.
+    destruct H.
+    {
+      unfold inDlyBuff in H.
+      simpls.
+      simpljoin1.
+      destruct H.
+      {
+        inversion H; subst.
+        right.
+        eapply regdlySt_cons_same; eauto.
+      }
+      {
+        left.
+        unfold inDlyBuff.
+        simpl; eauto.
+      }
+    }
+    {
+      right; eauto.
+    }
+Qed.
+
+Lemma regdlySt_notin_subst_sable :
+  forall t s0 w w0 M R F D D' d,
+    regdlySt t s0 w (M, (R, F), (d, s0, w0) :: D) ->
+    noDup (s0 :: getRegs D') ->
+    regdlySt t s0 w (M, (R, F), (d, s0, w0) :: D').
+Proof.
+  intro t.
+  induction t; intros.
+  -
+    simpls.
+    unfolds inDlyBuff.
+    simpljoin1.
+    simpl in H.
+    destruct H.
+    {
+      inversion H; subst.
+      simpl; eauto.
+    }
+    {
+      simpl in H1.
+      inversion H1; subst.
+      eapply dlyitem_in_dlyls_reg_in in H; eauto.
+      tryfalse.
+    }
+  -
+    simpls.
+    destruct H.
+    {
+      left.
+      unfolds inDlyBuff.
+      simpls.
+      simpljoin1.
+      destruct H.
+      inversion H; subst; eauto.
+      inversion H1; subst; eauto.
+      eapply dlyitem_in_dlyls_reg_in in H; eauto.
+      tryfalse.
+    }
+    {
+      eauto.
+    }
+Qed.
+    
+Lemma inregdly_exe_dly_stable :
+  forall D R' D' F t (s : SpReg) w x,
+    (R', D') = exe_delay (RegMap.set s (Some x) empR) D ->
+    regdlySt t s w (empM, (RegMap.set s (Some x) empR, F), D) ->
+    (empM, (R', F), D') |= t @ s |==> w.
+Proof.
+  intro D.
+  induction D; intros.
+  -
+    simpl in H.
+    simpl in H.
+    simpls.
+    inversion H; subst.
+    exists x.
+    repeat (split; eauto).
+  -    
+    destruct a, p.
+    simpl in H.
+    destruct d.
+    {
+      destruct (exe_delay (RegMap.set s (Some x) empR) D) eqn:Heqe; eauto.
+      inversion H; subst.
+      symmetry in Heqe. 
+      destruct (sep_reg_dec s s0) eqn:Heqe1.
+      {
+        subst.
+        lets Ht : H0.
+        eapply regdlySt_in_vl_eq in H0; eauto.
+        subst.
+        simpl.
+        exists w0.
+        repeat (split; eauto).
+        symmetry in Heqe.
+        eapply reg_not_in_dlybuff_exe_dly_stable in Heqe; eauto.
+        subst.
+        rewrite indom_setR_eq_RegMap_set; eauto.
+        rewrite regset_twice; eauto.
+        eapply regset_l_l_indom; eauto.
+        eapply regdlySt_cons_notin in Ht; eauto.
+        symmetry in Heqe.
+        lets Hexe_dly : Heqe.
+        eapply reg_not_in_dlybuff_exe_dly_stable in Heqe; eauto.
+        subst.
+        right.
+        unfold regSt.
+        simpl.
+        repeat (split; eauto).
+        rewrite indom_setR_eq_RegMap_set; eauto.
+        rewrite regset_twice; eauto.
+        eapply regset_l_l_indom; eauto. 
+        eapply regdlySt_cons_notin in Ht; eauto.
+        eapply not_in_exe_dly_stable in Ht; eauto.
+        eapply regdlySt_cons_notin in Ht; eauto.
+      }
+      { 
+        eapply regdlySt_noteq_cons_remove in H0; eauto.
+        eapply IHD with (R' := r) (D' := d) in H0; eauto.
+        clear - H0 n. 
+        simpls.
+        simpljoin1.
+        exists x.
+        repeat (split; eauto).
+        eapply not_indom_set_R_stable; eauto.
+        intro.
+        clear - n H.
+        unfold indom in *.
+        simpljoin1.
+        unfolds RegMap.set.
+        destruct_rneq_H.
+        destruct H1.
+        left.
+        rewrite not_indom_set_R_stable; eauto.
+        intro.
+        clear - n H0.
+        unfold indom in *.
+        simpljoin1.
+        unfolds RegMap.set.
+        destruct_rneq_H.
+        right.
+        rewrite not_indom_set_R_stable; eauto.
+        intro.
+        clear - n H0.
+        unfold indom in H0.
+        simpljoin1.
+        unfolds RegMap.set.
+        destruct_rneq_H.
+      }
+    }
+    {
+      destruct (exe_delay (RegMap.set s (Some x) empR) D) eqn:Heqe.
+      inversion H; subst.
+      destruct (sep_reg_dec s s0) eqn:Heqe1.
+      { 
+        subst.
+        lets Ht : Heqe. 
+        eapply reg_not_in_dlybuff_exe_dly_stable in Heqe; eauto.
+        subst.
+        simpl.
+        exists x.
+        repeat (split; eauto). 
+        left. 
+        lets Hregdly : H0. 
+        eapply regdlySt_dlytim_reduce_stable in H0; eauto.
+        eapply regdlySt_notin_subst_sable; eauto. 
+        eapply regdlySt_noDup in H0; eauto.
+        simpl in H0.
+        inversion H0; subst.
+        eapply noDup_exe_dly_stable in H4; eauto.
+        econstructor; eauto.
+        eapply not_in_exe_dly_stable in H3; eauto.
+        eapply regdlySt_cons_notin in H0; eauto.
+      }
+      {
+        lets Hexe_delay : Heqe.
+        lets Hnodup : H0.
+        eapply regdlySt_noDup in Hnodup; eauto. simpl in Hnodup.
+        inversion Hnodup; subst. 
+        eapply not_in_exe_dly_stable in Heqe; eauto.
+        eapply regdlySt_noteq_cons_remove in H0; eauto.  
+        eapply IHD with (R' := r) (D' := d0) in H0; eauto. 
+        clear - H0 n Heqe.
+        simpls.
+        simpljoin1.
+        exists x.
+        repeat (split; eauto).
+        destruct H1.
+        left.  
+        eapply regdlySt_cons_noteq_stable in H; eauto.
+        right.
+        unfolds regSt.
+        simpls.
+        simpljoin1.
+        repeat (split; eauto).
+        intro. 
+        eapply H1.
+        destruct H0.
+        subst; tryfalse.
+        eauto.
+      }
+    }
+Qed.
+    
+Lemma dlytime_gt_zero_reduce_exe_dly :
+  forall D M R R' D' F t s w,
+    (M, (R, F), D) |= S t @ s |==> w ->
+    (R', D') = exe_delay R D ->
+    (M, (R', F), D') |= t @ s |==> w.
+Proof.
+  intros.
+  lets Ht : H.
+  simpl in Ht.
+  simpljoin1.
+
+  destruct H3.
+  { 
+    destruct H1.
+    {
+      eapply dlytm_gt_zero_exe_dly; eauto.
+    }
+    {
+      eapply inregdly_exe_dly_stable; eauto.
+    }
+  }
+  {
+    assert ((empM, (RegMap.set s (Some x) empR, F), D) |= s |=> w).
+    {
+      simpl.
+      eauto.
+    }
+
+    eapply dly_reduce_reg_stable in H2; eauto.
+    eapply regst_conseq_regdly; eauto.
+  }
+Qed.
+  
+Lemma dly_reduce_dlyreg_stable :
+  forall D M R R' F D' s w n,
+    (M, (R, F), D) |= n @ s |==> w ->
+    (R', D') = exe_delay R D ->
+    (M, (R', F), D') |= (n @ s |==> w ↓).
+Proof.
+  intros.
+  destruct n.
+  { 
+    simpl TimReduce.
+    eapply dlytime_zero_exe_dly; eauto.
+  }
+  {
+    simpl TimReduce.
+    eapply dlytime_gt_zero_reduce_exe_dly; eauto.
+  }
+Qed.
+
+Lemma Afrmlist_exe_delay_stable :
+  forall D D' M R R' F w f,
+    (M, (R, F), D) |= {|w, f|} ->
+    (R', D') = exe_delay R D ->
+    (M, (R', F), D') |= {|w, f|}.
+Proof.
+  intro D.
+  induction D; intros.
+  -
+    simpls.
+    simpljoin1.
+    repeat (split; eauto).
+  -
+    destruct a, p.
+    assert ((M, (R, F), D) |= {|w, f|}).
+    {
+      clear - H.
+      simpls.
+      simpljoin1.
+      split; eauto.
+    }
+    simpl in H0.
+    destruct d.
+    {
+      destruct (exe_delay R D) eqn:Heqe.
+      inversion H0; subst.
+      symmetry in Heqe.
+      eapply IHD with (R' := r) (D' := d) in H1; eauto.
+      clear - H1.
+      simpls.
+      simpljoin1.
+      split; eauto.
+      unfolds regSt.
+      simpls.
+      simpljoin1.
+      repeat (split; eauto).
+      rewrite not_indom_set_R_stable; eauto.
+      intro.
+      unfold indom in *.
+      simpljoin1.
+      unfolds RegMap.set.
+      destruct_rneq_H.
+    }
+    {
+      destruct (exe_delay R D) eqn:Heqe.
+      inversion H0; subst.
+      symmetry in Heqe.
+      eapply IHD with (R' := r) (D' := d0) in H1; eauto.
+    }
+Qed.
+
+Lemma exe_dly_sep_split :
+  forall D R1 R2 R' D',
+    exe_delay (merge R1 R2) D = (R', D') -> disjoint R1 R2 ->
+    exists R1' R2', R' = merge R1' R2' /\ disjoint R1' R2' /\
+               exe_delay R1 D = (R1', D') /\ exe_delay R2 D = (R2', D').
+Proof.
+  intro D.
+  induction D; intros.
+  -
+    simpl in H.
+    inversion H; subst.
+    exists R1 R2.
+    repeat (split; eauto).
+  -
+    destruct a, p.
+    simpl in H.
+    destruct d.
+    {
+      destruct (exe_delay (R1 ⊎ R2) D) eqn:Heqe.
+      inversion H; subst.
+      eapply IHD in Heqe; eauto.
+      simpljoin1.
+      renames x to R1', x0 to R2'.
+
+      destruct (indom_nor_not s R1').
+      {
+        exists (set_R R1' s w) R2'.
+        repeat (split; eauto).
+        rewrite indom_setR_eq_RegMap_set; eauto.
+        rewrite indom_setR_eq_RegMap_set; eauto. 
+        rewrite indom_setR_merge_eq; eauto.
+        eapply indom_merge_still; eauto.
+        simpl.
+        eapply disjoint_setR_still1; eauto.
+        simpl.
+        rewrite H3; eauto.
+        simpl.
+        rewrite H4; eauto.
+        eapply indom_m1_disj_notin_m2 with (l := s) in H2; eauto.
+        rewrite not_indom_set_R_stable; eauto.
+      }
+      {
+        exists R1' (set_R R2' s w).
+        repeat (split; eauto).  
+        rewrite indom_setR_merge_eq2; eauto. 
+        eapply disjoint_setR_still2; eauto.
+        simpl.
+        rewrite H3; eauto.
+        rewrite not_indom_set_R_stable; eauto.
+        simpl.
+        rewrite H4; eauto.
+      }
+    }
+    {
+      destruct (exe_delay (R1 ⊎ R2) D) eqn:Heqe.
+      inversion H; subst.
+      eapply IHD in Heqe; eauto.
+      simpljoin1.
+      renames x to R1', x0 to R2'.
+      exists R1' R2'.
+      repeat (split; eauto).
+      simpl.
+      rewrite H3; eauto.
+      simpl.
+      rewrite H4; eauto.
+    }
+Qed.
+    
+Lemma dly_reduce_asrt_stable :
+  forall p M R R' F D D',
+    (M, (R, F), D) |= p -> (R', D') = exe_delay R D ->
+    (M, (R', F), D') |= (p ↓).
+Proof.
+  intros p.
+  induction p; intros.
+
+  - (* Aemp *)
+    simpl TimReduce. 
+    eapply dly_reduce_Aemp_stable; eauto.
+
+  - (* Amapsto *)
+    simpl TimReduce.
+    eapply dly_reduce_Amapsto_stable; eauto.
+  
+  - (* Aaexp *)
+    simpl TimReduce.
+    eapply dly_reduce_Aaexp_stable; eauto.
+
+  - (* Aoexp *)
+    simpl TimReduce.
+    eapply dly_reduce_Aoexp_stable; eauto.
+
+  - (* regst *)
+    simpl TimReduce.
+    eapply dly_reduce_reg_stable; eauto.
+
+  - (* dlyregst *)
+    eapply dly_reduce_dlyreg_stable; eauto.
+
+  - (* APure *)
+    simpl TimReduce.
+    simpls; eauto.
+ 
+  - (* AframeList *)
+    simpl TimReduce.
+    eapply Afrmlist_exe_delay_stable; eauto.
+
+  - (* Atrue *)
+    simpl TimReduce.
+    simpls; eauto.
+
+  - (* Afalse *)
+    simpl TimReduce.
+    simpls; eauto.
+
+  - (* Aconj *)
+    simpl TimReduce.
+    simpl in H. simpl.
+    simpljoin1; eauto.
+
+  - (* Adisj *)
+    simpl TimReduce.
+    simpl in H. simpl.
+    destruct H; eauto.
+
+  - (* Astar *)
+    sep_star_split_tac.
+    simpl in H4.
+    simpljoin1.
+    simpl TimReduce.
+    symmetry in H0.
+    eapply exe_dly_sep_split in H0; eauto.
+    simpljoin1.
+    renames x to r', x0 to r0'.
+    simpl.
+    exists (m, (r', f0), D') (m0, (r0', f0), D').
+    simpl.
+    repeat (split; eauto).
+
+  - (* Aforall *)
+    simpl in H0.
+    simpl.
+    intros.
+    specialize (H0 x).
+    eauto.
+
+  - (* Aexists *)
+    simpl in H0.
+    simpljoin1.
+    simpl.
+    exists x.
+    eauto.
 Qed.
 
 (*+ Lemmas about instruction +*)
